src/proof/DR.v
@@ -1,0 +1,83 @@
+Require Import List.
+Import ListNotations.
+
+Require Import sflib.
+
+From Memento Require Import Utils.
+From Memento Require Import Syntax.
+From Memento Require Import Semantics.
+From Memento Require Import Env.
+From Memento Require Import Common.
+
+Set Implicit Arguments.
+
+Definition DR (env: Env.t) (s: list Stmt) :=
+  forall tr tr' thr thr' thr_term thr_term' ts mmts,
+    thr = Thread.mk s [] ts mmts ->
+    thr' = Thread.mk s [] ts thr_term.(Thread.mmts) ->
+    Thread.rtc env tr thr thr_term [] ->
+    Thread.rtc env tr' thr' thr_term' [] ->
+  exists tr_x s_x c_x ts_x,
+    Thread.rtc env tr_x thr (Thread.mk s_x c_x ts_x thr_term'.(Thread.mmts)) []
+    /\ tr_x ~ tr ++ tr'
+    /\ (STOP thr_term.(Thread.stmt) thr_term.(Thread.cont) ->
+          thr_term.(Thread.stmt) = s_x
+          /\ thr_term.(Thread.cont) = c_x
+          /\ thr_term.(Thread.ts) = ts_x
+          /\ thr_term.(Thread.mmts) = thr_term'.(Thread.mmts)
+          /\ [] ~ tr')
+    /\ (STOP thr_term'.(Thread.stmt) thr_term'.(Thread.cont) ->
+          thr_term'.(Thread.stmt) = s_x
+          /\ thr_term'.(Thread.cont) = c_x
+          /\ thr_term'.(Thread.ts) = ts_x)
+  .
+
+Lemma DR_RW :
+  forall env envt labs s,
+    TypeSystem.judge env envt ->
+    EnvType.judge envt labs s ->
+    (* TODO: forall function *)
+  DR env s.
+Proof.
+  intros env envt labs s TYPEJ ENVTJ.
+  intros tr tr' thr thr' thr_term thr_term' ts mmts THR THR' EX1 EX2.
+  induction ENVTJ.
+  - eexists []. eexists s. eexists []. eexists ts.
+    inv EX1; ss; cycle 1.
+    { inv STEP. inv STEP0. inv STEP. ss. }
+    inv EX2; ss; cycle 1.
+    { inv STEP. inv STEP0. inv STEP. ss. }
+    splits; eauto.
+    + apply Thread.rtc_refl; eauto.
+    + apply refine_empty; eauto.
+    + i. splits; eauto. apply refine_empty; eauto.
+  - eexists []. eexists s. eexists []. eexists ts.
+    inv EX1; ss; cycle 1.
+    { inv STEP. inv STEP0. inv STEP. ss. }
+    inv EX2; ss; cycle 1.
+    { inv STEP. inv STEP0. inv STEP. ss. }
+    splits; eauto.
+    + apply Thread.rtc_refl; eauto.
+    + apply refine_empty; eauto.
+    + i. splits; eauto. apply refine_empty; eauto.
+  - eexists []. eexists s. eexists []. eexists ts.
+    inv EX1; ss; cycle 1.
+    { inv STEP. inv STEP0. inv STEP. ss. }
+    inv EX2; ss; cycle 1.
+    { inv STEP. inv STEP0. inv STEP. ss. }
+    splits; eauto.
+    + apply Thread.rtc_refl; eauto.
+    + apply refine_empty; eauto.
+    + i. splits; eauto. apply refine_empty; eauto.
+  - eexists []. eexists s. eexists []. eexists ts.
+    inv EX1; ss; cycle 1.
+    { inv STEP. inv STEP0. inv STEP. ss. }
+    inv EX2; ss; cycle 1.
+    { inv STEP. inv STEP0. inv STEP. ss. }
+    splits; eauto.
+    + apply Thread.rtc_refl; eauto.
+    + apply refine_empty; eauto.
+    + i. splits; eauto. apply refine_empty; eauto.
+  - admit.
+  - admit.
+Qed.
